define a good version of filter_query for LightFilter; prove lemmas to test the definition is correct

examples/sbf/LightFilter.v
@@ -15,6 +15,7 @@ Context {header_type : Set}.
 Context (num_frames num_rows num_slots frame_time : Z).
 Hypothesis H_num_slots : 0 < num_slots.
 Hypothesis H_num_rows : 0 < num_rows.
+Hypothesis H_num_frames : 2 <= num_frames.
 Context (hashes : list (header_type -> Z)).
 Hypothesis H_Zlength_hashes : Zlength hashes = num_rows.
 Hypothesis H_hashes : Forall (fun hash => forall h, 0 <= hash h < num_slots) hashes.
@@ -31,6 +32,7 @@ Definition filter := option (@filter header_type).
 Notation abs_insert := (@filter_insert header_type num_frames num_slots frame_time tick_time).
 Notation abs_query := (@filter_query header_type num_frames num_slots frame_time hashes tick_time).
 Notation abs_clear := (@filter_clear header_type num_frames num_slots frame_time tick_time).
+Notation abs_refresh := (@filter_refresh header_type num_frames num_slots frame_time tick_time).
 
 (* The time of guaranteed query, e.g. 59s. *)
 Definition T := frame_time * (num_frames - 2).
@@ -44,6 +46,8 @@ Axiom Tc_mul_num_slots_ge_frame_time : Tc * num_slots >= frame_time.
 Axiom Tc_le_tick_time : Tc <= tick_time.
 Lemma Tc_le_frame_time : Tc <= frame_time.
 Admitted.
+Lemma Tc_le_T : Tc <= frame_time.
+Admitted.
 
 Definition filter_insert (f : filter) (th : Z * header_type) : filter :=
   match f with
@@ -51,11 +55,16 @@ Definition filter_insert (f : filter) (th : Z * header_type) : filter :=
   | None => None
   end.
 
-(* TODO this is incorrect. *)
-Definition filter_query (f : filter) (th : Z * header_type) : option bool :=
+Definition filter_query (f : filter) '((t, h) : Z * header_type) : option bool :=
   match f with
-  | Some f =>
-      option_map snd (abs_query f th)
+  | Some (mk_filter window_hi last_timestamp num_clears normal_frames) =>
+      if last_timestamp <=? t then
+        let num_invalid_frames := Z.min (Z.max ((t - window_hi) / frame_time + 1) 0) (num_frames - 1) in
+        let valid_frames := sublist num_invalid_frames (num_frames - 1) normal_frames in
+        let res := existsb (fun hs => forallb (fun hash => fold_orb (map (Z.eqb (hash h) ∘ hash) hs)) hashes) valid_frames in
+        Some res
+      else
+        None
   | None => None
   end.
 
@@ -68,58 +77,105 @@ Definition filter_clear (f : filter) (t : Z) : filter :=
 
 (* Axiom filter_empty : filter. *)
 
-Definition ok_until (f : filter) (t : Z) : Prop :=
+Definition weak_filter_inv (f : filter) : Prop :=
   match f with
   | Some (mk_filter window_hi last_timestamp num_clears normal_frames) =>
-      0 <= t - last_timestamp <= Tc /\
-        last_timestamp < window_hi /\
-        (window_hi - 1 - last_timestamp) / Tc + num_clears >= num_slots
+      window_hi - frame_time <= last_timestamp < window_hi /\
+      Zlength normal_frames = num_frames - 1
   | None => False
   end.
 
-Lemma query_clear : forall f t t' h b,
-  ok_until f t ->
-  filter_query f (t', h) = Some b ->
-  filter_query (filter_clear f t) (t', h) = Some b.
-Proof.
-  intros.
-Admitted.
+Definition filter_inv (f : filter) : Prop :=
+  match f with
+  | Some (mk_filter window_hi last_timestamp num_clears normal_frames) =>
+      last_timestamp < window_hi /\
+      (window_hi - 1 - last_timestamp) / Tc + num_clears >= num_slots /\
+      Zlength normal_frames = num_frames - 1
+  | None => False
+  end.
 
-Lemma query_insert_same : forall f t t' h,
-  t <= t' < t+T ->
-  ok_until f t ->
-  filter_query (filter_insert f (t, h)) (t', h) = Some true.
-Admitted.
+Definition ok_until (f : filter) (t : Z) : Prop :=
+  (* filter_inv f /\ *)
+  match f with
+  | Some (mk_filter window_hi last_timestamp num_clears normal_frames) =>
+      0 <= t - last_timestamp <= Tc /\ filter_inv f
+        (* last_timestamp < window_hi /\
+        (window_hi - 1 - last_timestamp) / Tc + num_clears >= num_slots *)
+  | None => False
+  end.
 
-Lemma query_insert_other : forall f t t' h h',
-  ok_until f t ->
-  filter_query f (t', h') = Some true ->
-  filter_query (filter_insert f (t, h)) (t', h') = Some true.
-Admitted.
+Definition weak_filter_inv1 (f : filter) (new_timestamp : Z) : Prop :=
+  match f with
+  | Some (mk_filter window_hi last_timestamp num_clears normal_frames) =>
+      window_hi - frame_time <= new_timestamp < window_hi /\
+      Zlength normal_frames = num_frames - 1
+  | None => False
+  end.
 
-Lemma ok_insert : forall f t t' h,
-  t <= t' <= t + Tc ->
-  ok_until f t ->
-  ok_until (filter_insert f (t, h)) t'.
-Admitted.
-
-Notation abs_refresh := (@filter_refresh header_type num_frames num_slots frame_time tick_time).
+Definition filter_inv1 (f : filter) (new_timestamp : Z) : Prop :=
+  match f with
+  | Some (mk_filter window_hi last_timestamp num_clears normal_frames) =>
+      new_timestamp < window_hi /\
+      (window_hi - 1 - new_timestamp) / Tc + (num_clears + 1) >= num_slots /\
+      Zlength normal_frames = num_frames - 1
+  | None => False
+  end.
 
 Definition ok_until1 (f : filter) (new_timestamp : Z) (t : Z) : Prop :=
   match f with
   | Some (mk_filter window_hi _ num_clears normal_frames) =>
-      0 <= t - new_timestamp <= Tc /\
-        new_timestamp < window_hi /\
-        (window_hi - 1 - new_timestamp) / Tc + (num_clears + 1) >= num_slots
+      0 <= t - new_timestamp <= Tc /\ filter_inv1 f new_timestamp
+        (* new_timestamp < window_hi /\
+        (window_hi - 1 - new_timestamp) / Tc + (num_clears + 1) >= num_slots *)
   | None => False
   end.
+
+Lemma inv_refresh : forall f t,
+  ok_until (Some f) t ->
+  filter_inv1 (abs_refresh f t) t.
+Proof.
+Admitted.
+
+(* Definition low_inv (f : filter) : forall  *)
+
+Lemma weak_filter_inv1_abs_refresh : forall f t,
+  weak_filter_inv (Some f) ->
+  match abs_refresh f t with
+  | Some f =>
+      weak_filter_inv1 (Some f) t
+  | None => True
+  end.
+Admitted.
+
+(* filter_inv (abs_refresh f t) t. *)
+Lemma abs_query_pattern_ok : forall f t h f' res,
+  weak_filter_inv (Some f) ->
+  abs_query f (t, h) = Some (f', res) ->
+  filter_clear (Some f) t = Some f' /\ filter_query (filter_clear (Some f) t) (t, h) = Some res.
+Proof.
+  intros * ?H H_abs_query.
+  unfold filter_clear, filter_query, abs_clear, abs_query in *.
+  pose proof (weak_filter_inv1_abs_refresh f t ltac:(auto)).
+  destruct (abs_refresh f t) as [[window_hi last_timestamp num_clears normal_frames] | ].
+    2 : inv H_abs_query.
+  unfold weak_filter_inv1 in *.
+  assert ((t - window_hi) / frame_time + 1 = 0). {
+    rewrite <- Zdiv.Z_div_plus by lia.
+    apply Z.div_small; lia.
+  }
+  inv H_abs_query.
+  split; only 1 : auto.
+  replace (t <=? t) with true by lia.
+  f_equal. f_equal.
+  list_solve.
+Qed.
 
 Lemma ok_refresh : forall f t t',
   t <= t' <= t + Tc ->
   ok_until (Some f) t ->
   ok_until1 (abs_refresh f t) t t'.
 Proof.
-  intros * H_t' H_ok_until.
+  (* intros * H_t' H_ok_until.
   destruct f as [window_hi last_timestamp num_clears normal_frames].
   simpl in *.
   replace (last_timestamp <=? t) with true by lia.
@@ -141,8 +197,91 @@ Proof.
       admit.
     }
     rewrite Zdiv.Z_div_plus in * by admit.
-    lia.
+    lia. *)
 Admitted.
+
+Lemma query_clear : forall f t t' h b,
+  t <= t' ->
+  ok_until f t ->
+  filter_query f (t', h) = Some b ->
+  filter_query (filter_clear f t) (t', h) = Some b.
+Proof.
+  intros.
+Admitted.
+
+Lemma existsb_Znth_true : forall {A} {d : Inhabitant A} (f : A -> bool) l i,
+  0 <= i < Zlength l ->
+  f (Znth i l) = true ->
+  existsb f l = true.
+Proof.
+  induction l; intros.
+  - list_solve.
+  - destruct (i =? 0) eqn:?H.
+    + simpl.
+      replace (f a) with true by list_solve.
+      auto.
+    + specialize (IHl (i-1) ltac:(list_solve) ltac:(list_solve)).
+      simpl.
+      rewrite IHl.
+      destruct (f a); auto.
+Qed.
+
+Lemma query_insert_same : forall f t t' h,
+  t <= t' <= t+T ->
+  ok_until f t ->
+  filter_query (filter_insert f (t, h)) (t', h) = Some true.
+Proof.
+  intros * H_t' H_ok_until.
+  destruct f. 2 : inv H_ok_until.
+  unfold filter_insert, abs_insert.
+  pose proof (H_filter_inv1 := inv_refresh f t ltac:(auto)).
+  destruct (abs_refresh f t) as [f' | ] in *. 2 : inv H_filter_inv1.
+  destruct f'.
+  unfold filter_query, filter_inv1 in *.
+  replace (t <=? t') with true by lia.
+  assert ((t' - window_hi) / frame_time < num_frames - 2). {
+    apply Z.div_lt_upper_bound. 1 : lia.
+    fold T.
+    lia.
+  }
+  f_equal.
+  apply existsb_Znth_true with (i := num_frames - 2 - Z.max ((t' - window_hi) / frame_time + 1) 0).
+  { list_solve. }
+  rewrite forallb_fold_andb.
+  apply fold_andb_true; list_simplify; intros.
+  rewrite <- existsb_fold_orb.
+  list_simplify.
+  rewrite existsb_app.
+  simpl.
+  unfold compose.
+  replace (Znth i hashes h =? Znth i hashes h) with true by lia.
+  rewrite orbF.
+  rewrite orbT.
+  auto.
+Qed.
+
+Lemma query_insert_other : forall f t t' h h',
+  t <= t' ->
+  ok_until f t ->
+  filter_query f (t', h') = Some true ->
+  filter_query (filter_insert f (t, h)) (t', h') = Some true.
+Admitted.
+
+Lemma ok_insert : forall f t t' h,
+  t <= t' <= t + Tc ->
+  ok_until f t ->
+  ok_until (filter_insert f (t, h)) t'.
+Proof.
+  intros * H_t' H_ok_until.
+  destruct f. 2 : inv H_ok_until.
+  pose proof (H_ok_refresh := ok_refresh f t t' ltac:(auto) ltac:(auto)).
+  unfold filter_insert, abs_insert in *.
+  destruct (abs_refresh f t). 2 : inv H_ok_refresh.
+  destruct f0.
+  unfold ok_until, filter_inv.
+  rewrite Zlength_upd_Znth.
+  apply H_ok_refresh.
+Qed.
 
 Lemma ok_clear : forall f t t',
   t <= t' <= t + Tc ->
